Cartesian CuTT style fibrancy

theories/translation_fib.v
@@ -27,12 +27,6 @@ Admitted.
 
 Definition cofib (p : ℙ) := forall q (α : q ≤ p), precofib q.
 
-Definition lbox {p} : cofib p -> cofib (S p).
-Admitted.
-
-Definition rbox {p} : cofib p -> cofib (S p).
-Admitted.
-
 Definition is1 {p} : cofib p -> SProp.
 Admitted.
 
@@ -45,43 +39,36 @@ Definition is1_match {p} {X : Type} (c : cofib p)
   (b2 : (is1 c -> sFalse) -> X) : X.
 Admitted.
 
-Definition is1_promote_lbox {p q r} (α : q ≤ p) (β : r ≤ S q) (c : cofib p) : 
-  is1 (β ⋅ lbox (α ⋅ c)) -> is1 ((promote α) ∘ β ⋅ lbox c).
-Admitted.
-
-Definition is1_promote_rbox {p q r} (α : q ≤ p) (β : r ≤ S q) (c : cofib p) : 
-  is1 (β ⋅ rbox (α ⋅ c)) -> is1 ((promote α) ∘ β ⋅ rbox c).
-Admitted.
+Definition lid (p : ℙ) := p ≤ 1.
 
 (* welcome to fibrancy HELL *)
 Record FPsh@{i} : Type :=
 mkFPsh {
   fpsh0 : forall p : ℙ, Type@{i} ;
   fpsh1 : forall p : ℙ, (forall q (α : q ≤ p), fpsh0 q) -> SProp ;
-  fpshl0 : forall (p : ℙ) (c : cofib p)
-    (s0 : forall (q : ℙ) (α : q ≤ S p) (αε : is1 (α ⋅ lbox c)), fpsh0 q)
-    (s1 : forall (q : ℙ) (α : q ≤ S p) (αε : is1 (α ⋅ lbox c)), fpsh1 q (fun r β => s0 r (α ∘ β) (is1_funct β _ αε))),
+  fpshl0 : forall (p : ℙ) (c : cofib p) (l l' : lid p)
+    (s0 : forall (q : ℙ) (α : q ≤ S p) (αε : is1 (squish ∘ α ⋅ c)), fpsh0 q)
+    (s1 : forall (q : ℙ) (α : q ≤ S p) (αε : is1 (squish ∘ α ⋅ c)), fpsh1 q (fun r β => s0 r (α ∘ β) (is1_funct β _ αε)))
+    (l0 : forall (q : ℙ) (α : q ≤ p), fpsh0 q)
+    (l1 : forall (q : ℙ) (α : q ≤ p), 
+      fpsh1 q (fun r β => is1_match (α ∘ β ⋅ c)
+        (fun βε => s0 r ((merge ! l) ∘ α ∘ β) βε)
+        (fun _ => l0 r (α ∘ β)))),
     fpsh0 p ;
-  fpshl1 : forall (p : ℙ) (c : cofib p)
-    (s0 : forall (q : ℙ) (α : q ≤ S p) (αε : is1 (α ⋅ lbox c)), fpsh0 q)
-    (s1 : forall (q : ℙ) (α : q ≤ S p) (αε : is1 (α ⋅ lbox c)), fpsh1 q (fun r β => s0 r (α ∘ β) (is1_funct β _ αε))),
-    fpsh1 p (fun q α => is1_match ((side_1 ∘ α) ⋅ lbox c)
-      (fun αε => s0 q (side_1 ∘ α) αε)
-      (fun _ => fpshl0 q (α ⋅ c) 
-        (fun r β βε => s0 r (promote α ∘ β) (is1_promote_lbox α β c βε))
-        (fun r β βε => s1 r (promote α ∘ β) (is1_promote_lbox α β c βε)))) ;
-  fpshr0 : forall (p : ℙ) (c : cofib p)
-    (s0 : forall (q : ℙ) (α : q ≤ S p) (αε : is1 (α ⋅ rbox c)), fpsh0 q)
-    (s1 : forall (q : ℙ) (α : q ≤ S p) (αε : is1 (α ⋅ rbox c)), fpsh1 q (fun r β => s0 r (α ∘ β) (is1_funct β _ αε))),
-    fpsh0 p ;
-  fpshr1 : forall (p : ℙ) (c : cofib p)
-    (s0 : forall (q : ℙ) (α : q ≤ S p) (αε : is1 (α ⋅ rbox c)), fpsh0 q)
-    (s1 : forall (q : ℙ) (α : q ≤ S p) (αε : is1 (α ⋅ rbox c)), fpsh1 q (fun r β => s0 r (α ∘ β) (is1_funct β _ αε))),
-    fpsh1 p (fun q α => is1_match ((side_0 ∘ α) ⋅ rbox c)
-      (fun αε => s0 q (side_0 ∘ α) αε)
-      (fun _ => fpshr0 q (α ⋅ c) 
-        (fun r β βε => s0 r (promote α ∘ β) (is1_promote_rbox α β c βε))
-        (fun r β βε => s1 r (promote α ∘ β) (is1_promote_rbox α β c βε)))) ;
+  fpshl1 : forall (p : ℙ) (c : cofib p) (l l' : lid p)
+    (s0 : forall (q : ℙ) (α : q ≤ S p) (αε : is1 (squish ∘ α ⋅ c)), fpsh0 q)
+    (s1 : forall (q : ℙ) (α : q ≤ S p) (αε : is1 (squish ∘ α ⋅ c)), fpsh1 q (fun r β => s0 r (α ∘ β) (is1_funct β _ αε)))
+    (l0 : forall (q : ℙ) (α : q ≤ p), fpsh0 q)
+    (l1 : forall (q : ℙ) (α : q ≤ p), 
+      fpsh1 q (fun r β => is1_match (α ∘ β ⋅ c)
+        (fun βε => s0 r ((merge ! l) ∘ α ∘ β) βε)
+        (fun _ => l0 r (α ∘ β)))),
+    fpsh1 p (fun q α => is1_match (α ⋅ c)
+      (fun αε => s0 q ((merge ! l') ∘ α) αε)
+      (fun _ => fpshl0 q (α ⋅ c) (l ∘ α) (l' ∘ α)
+        (fun r β βε => s0 r (promote α ∘ β) βε)
+        (fun r β βε => s1 r (promote α ∘ β) βε)
+        (α ⋅ l0) (α ⋅ l1))) ;
 }.
 
 (* Elements of a presheaf *)
@@ -153,38 +140,35 @@ fun s => mkYtEl@{i j} q (yt_funct α f) (α ⋅ s.(ytel0)) (α ⋅ s.(ytel1)).
 Record yft@{i j} (p : ℙ) := mkYFT {
   yft0 : forall q (α : q ≤ p), Type@{i};
   yft1 : forall q (α : q ≤ p), (forall r (β : r ≤ q), yft0 r (α ∘ β)) -> SProp;
-  yftl0 : forall (q : ℙ) (α : S q ≤ p) (c : cofib q)
-    (s0 : forall (r : ℙ) (β : r ≤ S q) (βε : is1 (β ⋅ lbox c)), yft0 r (α ∘ β))
-    (s1 : forall (r : ℙ) (β : r ≤ S q) (βε : is1 (β ⋅ lbox c)), yft1 r (α ∘ β) (fun r0 β0 => s0 r0 (β ∘ β0) (is1_funct β0 _ βε))),
-    yft0 q (α ∘ side_1) ;
-  yftl1 : forall (q : ℙ) (α : S q ≤ p) (c : cofib q)
-    (s0 : forall (r : ℙ) (β : r ≤ S q) (βε : is1 (β ⋅ lbox c)), yft0 r (α ∘ β))
-    (s1 : forall (r : ℙ) (β : r ≤ S q) (βε : is1 (β ⋅ lbox c)), yft1 r (α ∘ β) (fun r0 β0 => s0 r0 (β ∘ β0) (is1_funct β0 _ βε))),
-    yft1 q (α ∘ side_1) (fun r (β : r ≤ q) => is1_match ((side_1 ∘ β) ⋅ lbox c)
-      (fun βε => s0 r (side_1 ∘ β) βε)
-      (fun _ => yftl0 r (α ∘ promote β) (β ⋅ c)
-        (fun r0 β0 β0ε => s0 r0 (promote β ∘ β0) (is1_promote_lbox β β0 c β0ε))
-        (fun r0 β0 β0ε => s1 r0 (promote β ∘ β0) (is1_promote_lbox β β0 c β0ε)))) ;
-  yftr0 : forall (q : ℙ) (α : S q ≤ p) (c : cofib q)
-    (s0 : forall (r : ℙ) (β : r ≤ S q) (βε : is1 (β ⋅ rbox c)), yft0 r (α ∘ β))
-    (s1 : forall (r : ℙ) (β : r ≤ S q) (βε : is1 (β ⋅ rbox c)), yft1 r (α ∘ β) (fun r0 β0 => s0 r0 (β ∘ β0) (is1_funct β0 _ βε))),
-    yft0 q (α ∘ side_0) ;
-  yftr1 : forall (q : ℙ) (α : S q ≤ p) (c : cofib q)
-    (s0 : forall (r : ℙ) (β : r ≤ S q) (βε : is1 (β ⋅ rbox c)), yft0 r (α ∘ β))
-    (s1 : forall (r : ℙ) (β : r ≤ S q) (βε : is1 (β ⋅ rbox c)), yft1 r (α ∘ β) (fun r0 β0 => s0 r0 (β ∘ β0) (is1_funct β0 _ βε))),
-    yft1 q (α ∘ side_0) (fun r (β : r ≤ q) => is1_match ((side_0 ∘ β) ⋅ rbox c)
-      (fun βε => s0 r (side_0 ∘ β) βε)
-      (fun _ => yftr0 r (α ∘ promote β) (β ⋅ c)
-        (fun r0 β0 β0ε => s0 r0 (promote β ∘ β0) (is1_promote_rbox β β0 c β0ε))
-        (fun r0 β0 β0ε => s1 r0 (promote β ∘ β0) (is1_promote_rbox β β0 c β0ε)))) ;
+  yftl0 : forall (q : ℙ) (α : S q ≤ p) (c : cofib q) (l l' : lid q)
+    (s0 : forall (r : ℙ) (β : r ≤ S q) (βε : is1 (squish ∘ β ⋅ c)), yft0 r (α ∘ β))
+    (s1 : forall (r : ℙ) (β : r ≤ S q) (βε : is1 (squish ∘ β ⋅ c)), yft1 r (α ∘ β) (fun r0 β0 => s0 r0 (β ∘ β0) (is1_funct β0 _ βε)))
+    (l0 : forall (r : ℙ) (β : r ≤ q), yft0 r (α ∘ (merge ! l) ∘ β))
+    (l1 : forall (r : ℙ) (β : r ≤ q), 
+      yft1 r (α ∘ (merge ! l) ∘ β) (fun r0 β0 => is1_match (β ∘ β0 ⋅ c)
+        (fun β0ε => s0 r0 ((merge ! l) ∘ β ∘ β0) β0ε)
+        (fun _ => l0 r0 (β ∘ β0)))),
+    yft0 q (α ∘ (merge ! l')) ;
+  yftl1 : forall (q : ℙ) (α : S q ≤ p) (c : cofib q) (l l' : lid q)
+    (s0 : forall (r : ℙ) (β : r ≤ S q) (βε : is1 (squish ∘ β ⋅ c)), yft0 r (α ∘ β))
+    (s1 : forall (r : ℙ) (β : r ≤ S q) (βε : is1 (squish ∘ β ⋅ c)), yft1 r (α ∘ β) (fun r0 β0 => s0 r0 (β ∘ β0) (is1_funct β0 _ βε)))
+    (l0 : forall (r : ℙ) (β : r ≤ q), yft0 r (α ∘ (merge ! l) ∘ β))
+    (l1 : forall (r : ℙ) (β : r ≤ q), 
+      yft1 r (α ∘ (merge ! l) ∘ β) (fun r0 β0 => is1_match (β ∘ β0 ⋅ c)
+        (fun β0ε => s0 r0 ((merge ! l) ∘ β ∘ β0) β0ε)
+        (fun _ => l0 r0 (β ∘ β0)))),
+    yft1 q (α ∘ (merge ! l')) (fun r β => is1_match (β ⋅ c)
+      (fun βε => s0 r ((merge ! l') ∘ β) βε)
+      (fun _ => yftl0 r (α ∘ promote β) (β ⋅ c) (l ∘ β) (l' ∘ β)
+        (fun r0 β0 β0ε => s0 r0 (promote β ∘ β0) β0ε)
+        (fun r0 β0 β0ε => s1 r0 (promote β ∘ β0) β0ε)
+        (β ⋅ l0) (β ⋅ l1))) ;
 }.
 
 Arguments yft0 {_}.
 Arguments yft1 {_}.
 Arguments yftl0 {_}.
 Arguments yftl1 {_}.
-Arguments yftr0 {_}.
-Arguments yftr1 {_}.
 
 Definition yft_funct@{i j} {p q : ℙ} (α : q ≤ p) :
   yft@{i j} p -> yft@{i j} q :=
@@ -194,8 +178,6 @@ fun f =>
   yft1 := α ⋅ yft1 f;
   yftl0 := α ⋅ yftl0 f;
   yftl1 := α ⋅ yftl1 f;
-  yftr0 := α ⋅ yftr0 f;
-  yftr1 := α ⋅ yftr1 f;
 |}.
 
 Definition yftR@{i j k} {p : ℙ} (s : forall q : nat, q ≤ p -> yft@{i j} q) : SProp :=
@@ -241,20 +223,15 @@ fun s => mkYftEl@{i j k} q (yft_funct α f) (α ⋅ s.(yftel0)) (α ⋅ s.(yftel
 Definition Uᶠ@{i j k l} : Psh@{l} :=
 mkPsh@{l} yft@{i j} (fun p s => yftR@{i j k} s).
 
-Definition Gluel {p : ℙ} 
-  (c : cofib p)
-  (s0 : forall q (α : q ≤ S p), is1 (α ⋅ lbox c) -> yft q)
-  (s1 : forall q (α : q ≤ S p) (αε : is1 (α ⋅ lbox c)),
-    yftR (fun r β => s0 r (α ∘ β) (is1_funct β (α ⋅ lbox c) αε))) :
-  yft p.
-Proof.
-Admitted.
-
-Definition Gluer {p : ℙ} 
-  (c : cofib p)
-  (s0 : forall q (α : q ≤ S p), is1 (α ⋅ rbox c) -> yft q)
-  (s1 : forall q (α : q ≤ S p) (αε : is1 (α ⋅ rbox c)),
-    yftR (fun r β => s0 r (α ∘ β) (is1_funct β (α ⋅ rbox c) αε))) :
+Definition Glue {p : ℙ} 
+  (c : cofib p) (l l' : lid p)
+  (s0 : forall q (α : q ≤ S p), is1 (squish ∘ α ⋅ c) -> yft q)
+  (s1 : forall q (α : q ≤ S p) (αε : is1 (squish ∘ α ⋅ c)),
+    yftR (fun r β => s0 r (α ∘ β) (is1_funct β _ αε)))
+  (l0 : forall q (α : q ≤ p), yft q)
+  (l1 : forall q (α : q ≤ p), yftR (fun r β => is1_match (α ∘ β ⋅ c)
+    (fun βε => s0 r (merge ! l ∘ α ∘ β) βε)
+    (fun _ => l0 r (α ∘ β)))) :
   yft p.
 Proof.
 Admitted.
@@ -264,21 +241,10 @@ Proof.
 unshelve econstructor.
 - exact (fun q α => yft q).
 - refine (fun q α s => yftR s).
-- refine (fun q α c s0 s1 => _).
-  refine (Gluel c s0 s1).
-- refine (fun q α c s0 s1 => _).
-  refine (Gluer c s0 s1).
-- refine (fun q α c s0 s1 r β => _). 
-  simpl in s0 ; simpl in s1.
+- refine (fun q α c l l' s0 s1 l0 l1 => _).
+  refine (Glue c l l' s0 s1 l0 l1).
+- refine (fun q α c l l' s0 s1 l0 l1 => _).
   apply sfalso.
-- refine (fun q α c s0 s1 r β => _). 
-  simpl in s0 ; simpl in s1.
-  apply sfalso.
-(*   unshelve econstructor.
-  + refine (fun r β => _). 
-    refine (is1_match (side_1 ∘ β ⋅ lbox c) (fun βε => _) (fun _ => _)).
-    * refine (yft0 (s0 r (side_1 ∘ β) βε) r !).
-    * apply falso. *)
 Defined.
 
 Definition U1 (p : ℙ) : psh1 Uᶠ p (fun q α => U0 q).
@@ -334,10 +300,8 @@ Proof.
 unshelve econstructor.
 - refine (fun r β => bool).
 - refine (fun r β s => boolR s).
-- refine (fun r β c s0 s1 => _). apply falso.
-- refine (fun r β c s0 s1 => _). apply falso.
-- refine (fun r β c s0 s1 => _). apply sfalso.
-- refine (fun r β c s0 s1 => _). apply sfalso.
+- refine (fun r β c l l' s0 s1 l0 l1 => _). apply falso.
+- refine (fun r β c l l' s0 s1 l0 l1 => _). apply sfalso.
 Defined.
 
 Definition bool1 {p} : @El1 p Type0 Type1 bool0.
@@ -381,10 +345,9 @@ unshelve econstructor.
   (B0 r (α ∘ β)).(yft1) r ! (fun r' β' => _)).
   unshelve refine (cast0 B0 B1 (α ∘ β) β' _).
   exact (f r' β' (β' · x0) (β' · x1)).
-- refine (fun r β c s0 s1 x0 x1 => _). apply falso.
-- refine (fun r β c s0 s1 x0 x1 => _). apply falso.
-- refine (fun r β c s0 s1 x0 x1 => _). apply sfalso.
-- refine (fun r β c s0 s1 x0 x1 => _). apply sfalso.
+- refine (fun r β c l l' s0 s1 l0 l1 x0 x1 => _).
+  simpl in *. apply falso.
+- refine (fun r β c l l' s0 s1 l0 l1 x0 x1 => _). apply sfalso.
 Defined.
 
 Definition Arr1 {p}
@@ -477,10 +440,8 @@ unshelve econstructor.
   exact (SigmaT (α ∘ β ⋅ A0) (α ∘ β ⋅ A1) (α ∘ β ⋅ P0) (α ∘ β ⋅ P1)).
 - refine (fun r β => _).
   exact (SigmaR (α ∘ β ⋅ A0) (α ∘ β ⋅ A1) (α ∘ β ⋅ P0) (α ∘ β ⋅ P1)).
-- refine (fun r β c s0 s1 => _). apply falso.
-- refine (fun r β c s0 s1 => _). apply falso.
-- refine (fun r β c s0 s1 => _). apply sfalso.
-- refine (fun r β c s0 s1 => _). apply sfalso.
+- refine (fun r β c l l' s0 s1 l0 l1 => _). apply falso.
+- refine (fun r β c l l' s0 s1 l0 l1 => _). apply sfalso.
 Defined.
 
 Definition Sigma1 {p}
@@ -770,10 +731,8 @@ unshelve econstructor.
     (fun r3 (β3 : r3 ≤ r) => B0 r3 (α ∘ β ∘ β3) (β3 · x0) (β3 · x1))
     (fun r3 (β3 : r3 ≤ r) => B1 r3 (α ∘ β ∘ β3) (β3 · x0) (β3 · x1))
     _ ! _ β2 (f0 r2 _ (β2 · x0) (β2 · x1))).
-- refine (fun r β c s0 s1 => _). apply falso.
-- refine (fun r β c s0 s1 => _). apply falso.
-- refine (fun r β c s0 s1 => _). apply sfalso.
-- refine (fun r β c s0 s1 => _). apply sfalso.
+- refine (fun r β c l l' s0 s1 l0 l1 x0 x1 => _). apply falso.
+- refine (fun r β c l l' s0 s1 l0 l1 x0 x1 => _). apply sfalso.
 Defined.
 
 Definition Prod1 {p}
@@ -890,10 +849,8 @@ unshelve econstructor.
   exact (cube_eq ((α ∘ β) · A0) ((α ∘ β) · A1) ((α ∘ β) · x0) ((α ∘ β) · y0)).
 - unshelve refine (fun r β s => _). simpl in s.
   exact (cube_eqR ((α ∘ β) · A0) ((α ∘ β) · A1) ((α ∘ β) · x0) ((α ∘ β) · y0) s).
-- refine (fun r β c s0 s1 => _). apply falso.
-- refine (fun r β c s0 s1 => _). apply falso.
-- refine (fun r β c s0 s1 => _). apply sfalso.
-- refine (fun r β c s0 s1 => _). apply sfalso.
+- refine (fun r β c l l' s0 s1 l0 l1 => _). apply falso.
+- refine (fun r β c l l' s0 s1 l0 l1 => _). apply sfalso.
 Defined.
 
 Definition eq1 {p}
